theories/tree_borrows/inv_accessors.v
@@ -15,6 +15,7 @@ Add Printing Constructor state item.
 Section lemmas.
   Context `{bor_stateGS Σ}.
   Local Notation bor_interp := (bor_interp sc_rel).
+  Local Notation bor_interp_inner := (bor_interp_inner sc_rel).
 
   Implicit Types
     (l : loc) (sc : scalar).
@@ -121,7 +122,7 @@ Section lemmas.
     move : Ha. apply is_fresh_block.
   Qed.
 
-  Lemma loc_controlled_alloc_update σ l' off sz n t (tk : tag_kind) sc :
+  Lemma loc_controlled_alloc_update Mcall σ l' off sz n t (tk : tag_kind) sc :
     let blk := fresh_block σ.(shp) in
     let l := (blk, 0) in
     let nt := σ.(snp) in
@@ -130,8 +131,8 @@ Section lemmas.
     let σ' := mkState h' α' σ.(scs) (S σ.(snp)) σ.(snc) in
     t ≠ nt →
     state_wf σ →
-    loc_controlled l' t tk sc σ →
-    loc_controlled l' t tk sc σ'.
+    loc_controlled Mcall l' t tk sc σ →
+    loc_controlled Mcall l' t tk sc σ'.
   Proof.
     intros blk l nt h' α' σ' Hnt Hwf Hcontrolled Hpre.
     assert (bor_state_pre l' t tk σ) as [Hown Hmem]%Hcontrolled.
@@ -349,13 +350,13 @@ Section lemmas.
     - rewrite Hmem. rewrite list_lookup_lookup_total; [done | ]. by apply lookup_lt_is_Some_2.
   Qed. *)
 
-  Lemma bor_interp_readN_target σ_t σ_s (t : tag) tk l v_t :
-    bor_interp σ_t σ_s -∗
+  Lemma bor_interp_readN_target σ_t σ_s M_call M_tag M_t M_s (t : tag) tk l v_t :
+    bor_interp_inner σ_t σ_s M_call M_tag M_t M_s -∗
     l ↦t∗[tk]{t} v_t -∗
     t $$ tk -∗
-    ⌜∀ i:nat, (i < length v_t)%nat → loc_controlled (l +ₗ i) t tk (v_t !!! i) σ_t⌝.
+    ⌜∀ i:nat, (i < length v_t)%nat → loc_controlled M_call (l +ₗ i) t tk (v_t !!! i) σ_t⌝.
   Proof.
-    iIntros "(% & % & % & % & (Hc & Htag_auth & Htag_t_auth & Htag_s_auth) & Hpub_cid & Hsrel & %Hcall & %Htag_interp & %Hwf_s & %Hwf_t)".
+    iIntros "((Hc & Htag_auth & Htag_t_auth & Htag_s_auth) & Hpub_cid & Hsrel & %Hcall & %Htag_interp & %Hwf_s & %Hwf_t)".
     iIntros "Hp Htag".
     iPoseProof (tkmap_lookup with "Htag_auth Htag") as "%Htag_lookup".
     destruct Htag_interp as (Htag_interp & _ & _).
@@ -367,13 +368,13 @@ Section lemmas.
     by apply lookup_lt_is_Some_2.
   Qed.
 
-  Lemma bor_interp_readN_source σ_t σ_s (t : tag) tk l v_s :
-    bor_interp σ_t σ_s -∗
+  Lemma bor_interp_readN_source σ_t σ_s M_call M_tag M_t M_s (t : tag) tk l v_s :
+    bor_interp_inner σ_t σ_s M_call M_tag M_t M_s -∗
     l ↦s∗[tk]{t} v_s -∗
     t $$ tk -∗
-      ⌜∀ i:nat, (i < length v_s)%nat → loc_controlled (l +ₗ i) t tk (v_s !!! i) σ_s⌝.
+      ⌜∀ i:nat, (i < length v_s)%nat → loc_controlled M_call (l +ₗ i) t tk (v_s !!! i) σ_s⌝.
   Proof.
-    iIntros "(% & % & % & % & (Hc & Htag_auth & Htag_t_auth & Htag_s_auth) & Hpub_cid & Hsrel & %Hcall & %Htag_interp & %Hwf_s & %Hwf_t)".
+    iIntros "((Hc & Htag_auth & Htag_t_auth & Htag_s_auth) & Hpub_cid & Hsrel & %Hcall & %Htag_interp & %Hwf_s & %Hwf_t)".
     iIntros "Hp Htag".
     iPoseProof (tkmap_lookup with "Htag_auth Htag") as "%Htag_lookup".
     destruct Htag_interp as (Htag_interp & _ & _).
@@ -913,13 +914,13 @@ Section lemmas.
   Qed.
   *)
   (** Dealloc lemmas *)
-  Lemma loc_controlled_dealloc_update σ l l' sz (α' : trees) (acc_tg lu_tg : tag) (tk : tag_kind) sc :
+  Lemma loc_controlled_dealloc_update Mcall σ l l' sz (α' : trees) (acc_tg lu_tg : tag) (tk : tag_kind) sc :
     apply_within_trees (memory_deallocate σ.(scs) acc_tg (l.2, sz)) l.1 σ.(strs)  = Some α' →
     state_wf σ →
     trees_contain acc_tg σ.(strs) l.1 →
     (acc_tg = lu_tg → l.1 = l'.1 → tk = tk_pub) →
-    loc_controlled l' lu_tg tk sc σ →
-    loc_controlled l' lu_tg tk sc (mkState (free_mem l sz σ.(shp)) (delete l.1 α') σ.(scs) σ.(snp) σ.(snc)).
+    loc_controlled Mcall l' lu_tg tk sc σ →
+    loc_controlled Mcall l' lu_tg tk sc (mkState (free_mem l sz σ.(shp)) (delete l.1 α') σ.(scs) σ.(snp) σ.(snc)).
   Proof.
     intros Hdealloc Hwf Hcontain Hpub Hcontrol Hpre.
     edestruct free_mem_lookup as [_ free_mem_lookup].
